ulib: partially complete arithmetic decision

ulib/FStar.Reflection.Formula.fst
@@ -28,41 +28,6 @@ let rec eqlist (f : 'a -> 'a -> bool) (xs : list 'a) (ys : list 'a) : Tot bool =
 
 let eq_qn = eqlist (fun s1 s2 -> String.compare s1 s2 = 0) 
 
-let rec collect_app' (args : list term) (t : term) : Tot (term * list term) (decreases t) =
-    match inspect t with
-    | Tv_App l r ->
-        collect_app' (r::args) l
-    | _ -> (t, args)
-let collect_app = collect_app' []
-
-let rec mk_app (t : term) (args : list term) : Tot term (decreases args) =
-    match args with
-    | [] -> t
-    | (x::xs) -> mk_app (pack (Tv_App t x)) xs
-
-val uncurry : ('a -> 'b -> 'c) -> ('a * 'b -> 'c)
-let uncurry f (x, y) = f x y
-
-val curry : ('a * 'b -> 'c) -> ('a -> 'b -> 'c)
-let curry f x y = f (x, y)
-
-val mk_app_collect_inv_s : (t:term) -> (args:list term) ->
-                            Lemma (uncurry mk_app (collect_app' args t) == mk_app t args)
-let rec mk_app_collect_inv_s t args =
-    match inspect t with
-    | Tv_App l r ->
-        mk_app_collect_inv_s l (r::args);
-        pack_inspect_inv t
-    | _ -> ()
-
-val mk_app_collect_inv : (t:term) -> Lemma (uncurry mk_app (collect_app t) == t)
-let rec mk_app_collect_inv t = mk_app_collect_inv_s t []
-
-(*
- * The way back is not stricly true: the list of arguments could grow.
- * It's annoying to even state, might do it later
- *)
-
 let term_view_as_formula (tv:term_view) : Tot formula =
     match tv with
     | Tv_Var n ->
@@ -103,8 +68,8 @@ let term_view_as_formula (tv:term_view) : Tot formula =
     | Tv_Const (C_Int i) ->
         IntLit i
 
-    // TODO: all these
-    | Tv_Type ()
+    // TODO: all these. Do we want to export them?
+    | Tv_Type _
     | Tv_Abs _ _
     | Tv_Refine _ _
     | Tv_Const (C_Unit)
