ulib/FStar.Reflection.Arith.fst
@@ -1,0 +1,54 @@
+module FStar.Reflection.Arith
+
+open FStar.Reflection.Syntax
+
+(*
+ * Simple decision procedure to decide if a term is an "arithmetic
+ * proposition", by which we mean a simple relation between two
+ * arithmetic expressions (each representing integers or naturals)
+ *
+ * Main use case: deciding, in a tactic, if a goal is an arithmetic
+ * expression and applying a custom decision procedure there (instead of
+ * feeding to the SMT solver)
+ *)
+
+type expr =
+    | Lit : int -> expr
+    | Sum   : expr -> expr -> expr
+    | Mult  : expr -> expr -> expr
+    | Neg   : expr -> expr
+    // | Div   : expr -> expr -> expr // Add this one?
+    | Atom : nat -> expr // uninterpreted atom
+
+type connective =
+    | Lt | Eq | Gt | Ne
+
+type prop = | MkProp : expr ->  connective -> expr -> prop
+
+let lt e1 e2 = MkProp e1 Lt e2
+let le e1 e2 = MkProp e1 Lt (Plus (Lit 1) e2)
+let eq e1 e2 = MkProp e1 Eq e2
+let ne e1 e2 = MkProp e1 Ne e2
+let gt e1 e2 = MkProp e1 Gt e2
+let ge e1 e2 = MkProp (Plus (Lit 1) e1) Gt e2
+
+(* Define a traversal monad! Makes exception handling and counter-keeping easy *)
+let tm a = nat -> option (a * nat)
+let return (x:'a) : tm 'a = fun i -> Some (x, i)
+let bind (m : tm 'a) (f : 'a -> tm 'b) : tm 'b = fun i -> match m i with
+                                                          | Some (x, j) -> f x j
+                                                          | None -> None
+let atom : tm nat = fun i -> Some (i, i + 1)
+let fail : tm 'a = fun i -> None
+
+val decide : term -> tm expr
+let rec decide t =
+    let hd, tl = collect_app t in
+    match inspect hd, tl with
+    | Tm_fvar fv, [l; r] ->
+        let qn = inspectfv fv in
+        if eq_qn qn add_qn then (l <-- decide l;
+                                 r <-- decide r;
+                                 return (Sum l r))
+        else fail
+    | _ -> fail
