ulib/FStar.Reflection.Syntax.Lemmas.fst
@@ -1,0 +1,26 @@
+module FStar.Reflection.Syntax.Lemmas
+
+open FStar.Reflection.Syntax
+
+val uncurry : ('a -> 'b -> 'c) -> ('a * 'b -> 'c)
+let uncurry f (x, y) = f x y
+
+val curry : ('a * 'b -> 'c) -> ('a -> 'b -> 'c)
+let curry f x y = f (x, y)
+
+val mk_app_collect_inv_s : (t:term) -> (args:list term) ->
+                            Lemma (uncurry mk_app (collect_app' args t) == mk_app t args)
+let rec mk_app_collect_inv_s t args =
+    match inspect t with
+    | Tv_App l r ->
+        mk_app_collect_inv_s l (r::args);
+        pack_inspect_inv t
+    | _ -> ()
+
+val mk_app_collect_inv : (t:term) -> Lemma (uncurry mk_app (collect_app t) == t)
+let rec mk_app_collect_inv t = mk_app_collect_inv_s t []
+
+(*
+ * The way back is not stricly true: the list of arguments could grow.
+ * It's annoying to even state, might do it later
+ *)
