ulib/FStar.Reflection.fst
@@ -1,4 +1,5 @@
 module FStar.Reflection
 
 include FStar.Reflection.Syntax
+include FStar.Reflection.Syntax.Lemmas
 include FStar.Reflection.Formula
